instructions/steps.md
@@ -12,12 +12,20 @@ diff=$(comm -23 $tmpdir/sort $tmpdir/check)
 [ -z "$diff" ] || (echo $diff && exit 1)
 -->
 
+Welcome! 
+We're going to take you through the process of implementing a simple function
+to parse an Amazon Resource Name (ARN) string
+in the verification-aware programming language Dafny.
+We're also going to use the Duvet code quality tool
+to ensure we comply with a human-readable specification of correctness.
+
 ## Step 1
 
-In VSCode open the directory `exercises/start`
-open the file `exercises/start/src/AwsKmsArnParsing.dfy`
+The `exercises/start` directory contains our initial state,
+with a few files to get you started.
 
-You should see
+In VS Code, open the file `exercises/start/src/AwsKmsArnParsing.dfy`,
+You should see:
 
 <!-- !test check prelude -->
 ```dafny
@@ -34,8 +42,12 @@ module {:options "-functionSyntax:4"} AwsKmsArnParsing {
 
 }
 
-
 ```
+
+You will also see the Dafny extension automatically download Dafny for you,
+if this is the first time you've opened a Dafny source file.
+
+Let's go over a few Dafny basics:
 
 1. `include` is how Dafny includes other files.
 The file `include.dfy` is a helper file we added for you.
@@ -47,7 +59,7 @@ Dafny does have ways to control what gets exported,
 but for now, lets just say everything is exported.
 
 1. `import` takes a named module
-and bring it into scope.
+and brings it into scope.
 
 1. `opened` takes all the exported names
 in the imported module and puts them in the current namespace.
@@ -55,10 +67,10 @@ This is where we will get symbols that don't exist in this file,
 for example `Split` and `Join`.
 
 1. `{:options "-functionSyntax:4"}`
-This is to simplify upgrading.
-When Dafny v4 is released modules with this option
-will "Just Work".
-If you are *really* interested:
+allows us to use the simplest syntax for function declarations,
+which will be the default in Dafny 4 once it is released.
+You can safely ignore this,
+but if you are *really* interested:
 see [Controlling language features
 ](https://dafny.org/dafny/DafnyRef/DafnyRef#sec-controlling-language) for more details.
 
@@ -66,26 +78,32 @@ see [Controlling language features
 
 Since we are dealing with correct software,
 we need a definition of correctness!
-We have given you a specification `aws-kms-key-arn.txt`.
-This has been lightly edited from [AWS Encryption SDK](https://github.com/awslabs/aws-encryption-sdk-specification/blob/master/framework/aws-kms/aws-kms-key-arn.md)
-for this workshop.
+We have given you a specification in `aws-kms-key-arn.txt`.
+This has been lightly edited from the [AWS Encryption SDK](https://github.com/awslabs/aws-encryption-sdk-specification/blob/master/framework/aws-kms/aws-kms-key-arn.md)
+for this workshop. This is no made-up problem we're solving!
+
+Take a minute to read the specification
+and understand what we're asking you to implement.
 
 Currently `duvet` is optimized to handle RFC style (ITEF) files.
 We have converted the markdown specification into this format for you.
 Soon, `duvet` will support markdown directly.
 
 `duvet` can read text documents
-and extract MUST/SHOULD ([RFC-2119](https://datatracker.ietf.org/doc/html/rfc2119) normative language) as requirements.
+and extract MUST/SHOULD ([RFC-2119](https://datatracker.ietf.org/doc/html/rfc2119) normative language) statements as requirements.
 `duvet` will keep track of these requirements for us.
 It will help us account every requirement,
-and ask us to provide some evidence that implemented requirements are correct.
-You will see how this work in more detail later.
+and ask us to provide some evidence that our implementation of the requirements are correct.
+You will see how this works in more detail later.
 
-In VSCode open a terminal and 
+In VS Code [open a terminal](https://code.visualstudio.com/docs/terminal/basics) and enter:
 
 ```bash
 cd exercises/start
 ````
+
+You can also right-click the `exercises/start` folder and click "Open in Integrated Terminal".
+
 
 Now let's extract the requirements and run a report.
 We have made nice `make` targets for you.
@@ -97,14 +115,20 @@ make duvet_report
 
 ```
 
-This fails because we have not even started.
-Open the `compliance_report.html` in a browser.
-You will see that we have a total of 20 requirements
+The second command fails because we have not even started.
+There will now be a `compliance_report.html` report in the `start` folder.
+Right-click it and select "Open with Live Server",
+which should open the page in your browser
+(in a separate tab if you are using the web version of VS Code).
+If you click on the `aws-kms-key-arn` link,
+you will see that we have a total of 20 requirements
 for our `aws-kms-key-arn` specification.
 
 Click on the specification and you can see details on these requirements.
 We will start on section `2.5` so go ahead
-and click on a 2.5 and take a second to read the specification.
+and click on one of the `2.5` links in the left-most column
+and take a minute to look at this part of the specification
+and how it breaks down into a checklist.
 
 ## Step 3
 
@@ -113,14 +137,23 @@ we need some containers to put the parts of the strings in.
 
 Paste the following code into the `AwsKmsArnParsing` module
 and then we will go over what it means.
+Assuming you are reading these steps on GitHub,
+there should be a handy hidden copy button
+in the top-right corner of each code snippet for your convenience and delight.
+Unless we say otherwise, each time we give you a snippet like this,
+go ahead and paste it into the correct place.
+You shouldn't see any errors,
+again unless we say otherwise.
+If you run into problems please 
+[cut us an issue](https://github.com/aws-samples/how-to-write-more-correct-software-workshop/issues/new)!
 
 ```dafny
 
   datatype AwsArn = AwsArn
   datatype AwsResource = AwsResource
 
-  predicate AwsArn?(arn:AwsArn)
-  predicate AwsResource?(resource:AwsResource)
+  predicate ValidAwsArn?(arn:AwsArn)
+  predicate ValidAwsResource?(resource:AwsResource)
   predicate AwsKmsArn?(arn:AwsArn)
   predicate AwsKmsResource?(resource:AwsResource)
 
@@ -135,9 +168,9 @@ To the right of the `=` are the `datatype`'s constructors.
 In this case, we have only one.
 Later we will have more.
 
-What is a `predicate` and what's the deal with that`?` at the end?
+What is a `predicate` and what's the deal with that `?` at the end?
 A `predicate` is a function that returns a `boolean`.
-It is syntactic sugar for `function AwsArn?(arn:AwsArn) : bool`.
+It is syntactic sugar for `function ValidAwsArn?(arn:AwsArn) : bool`.
 
 Generally such functions ask a question.
 For example "Is this AwsArn `arn` a valid AwsArn?".
@@ -151,7 +184,7 @@ We will use this later.
 ## Step 4
 
 Let's add some properties to our `datatype`s.
-Replace the two exicting `datatype`s with this.
+Replace the two existing `datatype`s with this.
 
 <!-- !test check container datatypes -->
 ```dafny
@@ -178,7 +211,7 @@ then `obj.service` is a `string`.
 
 `nameonly` forces callers to use named parameters.
 This makes the call more verbose,
-but it makes it much more readable.
+but also makes it much more readable.
 
 You are not required to use it
 in your code,
@@ -189,17 +222,17 @@ but I highly recommend it.
 Now we have some containers.
 Let's talk about the correct values for these containers.
 
-<!-- !test check AwsArn? -->
+<!-- !test check ValidAwsArn? -->
 ```dafny
 
-  predicate AwsArn?(arn:AwsArn)
+  predicate ValidAwsArn?(arn:AwsArn)
   {
     && arn.arnLiteral == "arn"
     && 0 < |arn.partition|
     && 0 < |arn.service|
     && 0 < |arn.region|
     && 0 < |arn.account|
-    && AwsResource?(arn.resource)
+    && ValidAwsResource?(arn.resource)
   }
 
 ```
@@ -207,16 +240,16 @@ Let's talk about the correct values for these containers.
 We are evaluating the `AwsArn` container
 to see if it is correct.
 We can read this `predicate` as:
-The arnLiteral MUST be the string "arn"
-and partition, service, region, and account
-MUST NOT be empty string
+The arnLiteral MUST be the string "arn";
+the partition, service, region, and account
+MUST NOT be empty strings;
 and finally the resource MUST be a correct AwsResource.
 
 A `predicate` is a kind of function.
 Functions in Dafny are just syntactic sugar for expressions.
 You will note that there is no `;`.
 The return value for any `predicate` or `function`
-is just the vary last unterminated expression.
+is just the value of the function's body.
 
 The leading token, `&&`, is just sugar.
 Leading boolean operators like this
@@ -230,17 +263,17 @@ So `0 < arn.partition.length`
 is probably how you would expect that to be written
 in a language you are more familiar with.
 
-We are calling `AwsResource?`
+We are calling `ValidAwsResource?`
 even though it does not have an implementation.
 If you tried to compile this,
 Dafny would complain.
-But all Dafny needs for `AwsArn?` to be valid
+But all Dafny needs for `ValidAwsArn?` to be valid
 is to be able to prove that it will always return a `bool`.
-Feel free to change `AwsResource?` to a function
+Feel free to change `ValidAwsResource?` to a function
 that returns something else and see :)
 
 ```dafny
-    function AwsResource?(resource: AwsResource): string
+    function ValidAwsResource?(resource: AwsResource): string
 ```
 
 ## Step 6
@@ -251,21 +284,21 @@ let's add implementations to our remaining three `predicate`s .
 <!-- !test check remaining correctness predicates -->
 ```dafny
 
-  predicate AwsResource?(resource:AwsResource)
+  predicate ValidAwsResource?(resource:AwsResource)
   {
     && 0 < |resource.value|
   }
 
   predicate AwsKmsArn?(arn:AwsArn)
   {
-    && AwsArn?(arn)
+    && ValidAwsArn?(arn)
     && arn.service == "kms"
     && AwsKmsResource?(arn.resource)
   }
 
   predicate AwsKmsResource?(resource:AwsResource)
   {
-    && AwsResource?(resource)
+    && ValidAwsResource?(resource)
     && (
       || resource.resourceType == "key"
       || resource.resourceType == "alias"
@@ -274,7 +307,8 @@ let's add implementations to our remaining three `predicate`s .
 
 ```
 
-Like `&&` is logical and, `||` is logical or.
+Just as `&&` is the logical "and" operator,
+`||` is the logical "or".
 So the resourceType for an `AwsKmsResource`
 MUST be either "key" or "alias".
 
@@ -285,10 +319,10 @@ Does this seem to capture most of what the specification says makes a valid AWS 
 
 Many languages have types similar to Dafny's `datatype`,
 albeit not always immutable.
-These types have a quality of correctness.
+These types already contribute some progress towards correctness.
 After all, you can't put a number into a string.
 
-A subset type lets us combine the correctness we defined
+A subset type in Dafny lets us combine the correctness we defined
 in our `predicate`s with a base `datatype`.
 We can then reason about this new type statically.
 If most types represent the basic shape of your data,
@@ -315,44 +349,36 @@ Let's create one!
 tells Dafny we want to define a type named `AwsKmsArn`.
 
 1. `arn: AwsArn` means that base type is `AwsArn`.
-To define the correctness of this `AwsArn`
-we need an instance that we can use.
+To define the constraints of this subset type,
+we need a symbol of the base type to use when defining these constraints.
 
-1. `| AwsKmsArn?(arn)` means that this instance `arn`
-MUST return `true` when passed to `AwsKmsArn?`.
-The `|` can be read as "such that".
-This type can be read
-"An `AwsKmsArn` is an `AwsArn` such that `AwsKmsArn?` is true"
+1. `| AwsKmsArn?(arn)` means that if we pass the instance `arn`
+   to `AwsKmsArn?`, it MUST return `true`.
+   The `|` can be read as "such that".
+   This type can be read
+   "An `AwsKmsArn` is an `AwsArn` `arn` such that `AwsKmsArn?(arn)` is true"
 
-Instead of a `predicate`
-Dafny will let us use any expression.
-So we could have inlined `AwsKmsArn?`.
-But it is simpler to prove
-that a given base type satisfies some constraints
-when they are wrapped up in a single `predicate`.
+   Instead of a `predicate`
+   Dafny will let us use any expression.
+   So we could have inlined `AwsKmsArn?`.
+   But it is simpler to prove
+   that a given base type satisfies some constraints
+   when they are wrapped up in a single `predicate`.
 
-1. `witness`
-In Dafny, types are generally expected to have some value.
-The `witness` is there to prove to Dafny
-that a value of this subset type can indeed exists.
-You can imagine that this could be valuable
-in the case of a complicated condition.
-But since in any event Dafny will REQUIRE
-that we prove any given value is correct,
-in our case we don't need this.
+1. `witness`:
+   In Dafny, some contexts only allow you to use a type
+   if you can prove at least one value of that type exists.
+   The `witness` clause is there to prove to Dafny
+   this is true, by providing a sample value.
+   In our case we don't need this.
 
-`witness *` tells Dafny,
-"Don't worry,
-it doesn't matter whether a value
-of this type actually exists."
+   `witness *` tells Dafny,
+   "Don't worry,
+   it doesn't matter whether a value
+   of this type actually exists."
 
-Dafny also has features
-where you can ask for a value of a given type.
-In these complicated cases
-Dafny may need help to understand how to create such a value.
-And the witness gives Dafny this information.
-Feel free to check out the [witness clauses](https://dafny.org/dafny/DafnyRef/DafnyRef#sec-witness)
-for more details.
+   Feel free to check out [witness clauses](https://dafny.org/dafny/DafnyRef/DafnyRef#sec-witness)
+   in the reference manual for more details.
 
 In the meantime,
 let's create a subset type for `AwsKmsResource`
@@ -375,7 +401,7 @@ with these naive signatures.
 
   function ParseAwsKmsArn(identifier: string)
     : (result: AwsKmsArn)
-  function ParseAwsKmsResources(identifier: string)
+  function ParseAwsKmsResource(identifier: string)
     : (result: AwsKmsResource)
 
 ```
@@ -384,20 +410,19 @@ with these naive signatures.
 However, `function`s in Dafny are more restrictive
 than you are probably used to.
 They are syntactic sugar for expressions.
-They are more like mathematical functions; 1000% deterministic.
+They are more like mathematical functions: 100% deterministic.
 The can't mutate, use loops, or create objects on the heap.
 These restrictions are important
-because `function` are the building blocks for proof.
-
+because `function`s are the building blocks for proof.
 They provide a good introduction to Dafny
 and we won't run into these restrictions today.
 
 `: (result: AwsKmsResource)`?
 The first `:` tells Dafny "This is the return value".
-By putting it in `()` we can give our return value a name.
-e.g. `result` and a type for this return value.
+By putting it in `()` we can give our return value a name
+(i.e. `result`) and a type for this return value.
 This lets us reference it in a postcondition or `ensures` clause.
-Postcondition are things that MUST be true
+Postconditions are things that MUST be true
 about the result of the function.
 We could have `: AwsKmsResource`.
 But for reasons beyond the scope of this workshop
@@ -406,8 +431,18 @@ the other is often preferred.
 ## Step 9
 
 Here is a naive first implementation.
-I'll note that it is `':'` not `":"`.
-The first is a character, the second is a string.
+Note that it is `':'` not `":"`:
+the first is a character, the second is a string.
+
+We have introduced the dreaded semicolon `;`,
+but never fear, we are still just defining a pure expression!
+This syntax is just a way of introducing names for sub-expressions.
+You can read `var x := e; y` as "let `x` be `e` within `y`".
+If you do this multiple times,
+you end up with something that looks suspiciously like
+a sequence of statements.
+Ultimately the result of the function
+is the expression following the last `;`.
 
 ```dafny
 
@@ -416,7 +451,7 @@ The first is a character, the second is a string.
   {
     var components := Split(identifier, ':');
 
-    var resource := ParseAwsKmsResources(components[5]);
+    var resource := ParseAwsKmsResource(components[5]);
 
     var arn := AwsArn(
       arnLiteral := components[0],
@@ -432,9 +467,10 @@ The first is a character, the second is a string.
 
 ```
 
-Now we see 2 problems.
-`index out of range` and
+Now we see two errors!
+`index out of range` on `components[5]`, and
 `value does not satisfy the subset constraints of 'AwsKmsArn'`
+on the final `arn`.
 
 Dafny does not believe us that `6 == |components|`.
 That is, that there are at least 5 `:` in `identifier`.
@@ -448,8 +484,10 @@ How can we ask Dafny about such things?
 Most languages have a way for you to do "console log debugging"
 where you make changes, run the code, and check the output.
 `assert` is a way to do something similar in Dafny.
-However, instead of checking specific value
-Dafny will check them all.
+However, instead of checking a specific value at runtime,
+Dafny will check them all before you ever execute your code.
+An `assert` is an error unless Dafny can deduce
+that it is impossible for the expression to be false.
 
 Generally `Split` functions will return a single element
 if the character does not appear in the string.
@@ -459,14 +497,15 @@ After the `Split` try adding
 ```dafny
     assert Split("no colon", ':') == ["no colon"];
 ```
-Dafny will indeed tell us that this is true!
+You should not see an error on this line,
+which is Dafny telling us that this is indeed true!
 
 This means we can
 ```dafny
     assert 1 <= |components|;
 ```
 and sure enough Dafny will believe us.
-But any larger number, say `assert 2 <= |components|;`
+But any larger number, say `assert 2 <= |components|;`,
 Dafny will disagree.
 
 <details><summary>Aside</summary>
@@ -493,19 +532,21 @@ before the above `assert`.
 ## Step 10
 
 Ok, so what do we do if there are not enough `:` in `identifier`?
-Dafny does not have a ability to `throw`.
+Dafny does not have a ability to `throw` an exception.
 The return type in Dafny is a contract or postcondition.
-That means that we MUST return an `AwsKmsArn`.
+That means that with the current function signature,
+we MUST return an `AwsKmsArn` no matter what.
 
 What we need is a way to express failure.
-Dafny has a way to do this,
-you can read about [failure compatible types here](https://dafny.org/dafny/DafnyRef/DafnyRef#sec-update-failure)
+Dafny has a way to do this.
+You can read about [failure compatible types here](https://dafny.org/dafny/DafnyRef/DafnyRef#sec-update-failure)
 if you like.
-But we will go over everything you need here.
+But we will go over everything you need.
 
 First we need a type that can express
 the difference between `Success` and `Failure`.
-In the `Wrappers` the `Result` type does exactly this.
+In the `Wrappers` module defined in the `Wrappers.dfy` file,
+the `Result` type does exactly this.
 It takes 2 type parameters.
 One for the `Success` and the other for `Failure`[^monad]
 
@@ -522,7 +563,7 @@ Update our function like so:
   {
     var components := Split(identifier, ':');
 
-    var resource := ParseAwsKmsResources(components[5]);
+    var resource := ParseAwsKmsResource(components[5]);
 
     var arn := AwsArn(
       arnLiteral := components[0],
@@ -546,7 +587,7 @@ Looking at our specification
 we see "A string with 5 ":" that delimit following 6 parts:".
 This means that we need `|components| == 5`.
 
-We could write
+We could write:
 ```dafny
 
   function ParseAwsKmsArn(identifier: string)
@@ -559,7 +600,7 @@ We could write
       Failure("Malformed arn: " + identifier)
     else
 
-      var resource := ParseAwsKmsResources(components[5]);
+      var resource := ParseAwsKmsResource(components[5]);
 
       var arn := AwsArn(
         arnLiteral := components[0],
@@ -577,7 +618,7 @@ We could write
 
 This is great!
 Dafny now believes us that `components[5]` will _always_ be valid.
-You can even ask Dafny `assert |components| < 7;` and it will object.
+You can even ask Dafny `assert 7 < |components|;` and it will object.
 But pretty quickly we are going to introduce a pyramid of doom
 as we continually indent for more and more each such condition.
 
@@ -599,7 +640,7 @@ Instead we will use
 
     :- Need(6 == |components|, "Malformed arn: " + identifier);
 
-    var resource := ParseAwsKmsResources(components[5]);
+    var resource := ParseAwsKmsResource(components[5]);
 
     var arn := AwsArn(
       arnLiteral := components[0],
@@ -615,11 +656,14 @@ Instead we will use
 
 ```
 
-`:-` is the Elephant operator,
-or ["Update with Failure"](https://dafny.org/dafny/DafnyRef/DafnyRef#sec-update-failure)
-It will look at the return value
-and if the return is `Success` it will extract the value,
-and if the return is `Failure` it will halt and return the error.
+`:-` is the Elephant symbol,
+used here in a ["Let or Fail" expression](https://dafny.org/dafny/DafnyRef/DafnyRef#2139-let-or-fail-expression).
+You can think of this as a drastically simplified model
+of throwing exceptions.
+It will first look at the value to the right of the `:-`:
+* If it is a `Success`, it will extract the value and evaluate the expression that follows the `;`. In this case, that means the remaining lines of the function body.
+* If it is a `Failure`, it will propagate that error as the result
+of the whole surrounding expression. In this case, that means the whole function body.
 
 In the case of `Need`,
 instead of a `Result` it returns an `Outcome`.
@@ -637,16 +681,19 @@ what you `Need` to be true to continue!
 Now, we _could_ annotate this `Need` line with duvet.
 But duvet wants both the implementation
 *and* evidence that it is correct.
-Dafny gives us an even more powerful too.
+Dafny gives us an even more powerful tool.
 Stay tuned.
 
 ## Step 12
 
-Now let's deal with
+Now let's deal with the remaining error,
 `value does not satisfy the subset constraints of 'AwsKmsArn'`.
+
+
 Since we stuffed all of the constraints
-of `AwsKmsArn` into a single predicate
+of `AwsKmsArn` into a single predicate,
 `:- Need(AwsKmsResource?(resource), "Malformed resource: " + identifier);`
+is all we need.
 
 ```dafny
 
@@ -657,7 +704,7 @@ of `AwsKmsArn` into a single predicate
 
     :- Need(6 == |components|, "Malformed arn: " + identifier);
 
-    var resource := ParseAwsKmsResources(components[5]);
+    var resource := ParseAwsKmsResource(components[5]);
 
     var arn := AwsArn(
       arnLiteral := components[0],
@@ -675,11 +722,14 @@ of `AwsKmsArn` into a single predicate
 
 ```
 
+Horray! Now Dafny is at least satisfied that the implementation
+of this function matches the signature and will not crash at runtime.
+
 ## Step 13
 
-Now we have an implementation let's review it for correctness.
+Now that we have a valid implementation, let's review it for correctness.
 Our first requirement is
-'A string with 5 ":" that MUST delimit following 6 parts:'.
+'A valid AWS KMS ARN is a string with 5 ":" that MUST delimit the following 6 parts:'.
 
 <!-- !test check ParseAwsKmsArn Correctness -->
 ```dafny
@@ -700,7 +750,7 @@ If Dafny can not prove them it will complain.
 so the computational overhead
 of many calls to `Split` will not exist in the compiled code.
 
-1. `.Success?`
+1. `.Success?`:
 Remember that `ParseAwsKmsArn` returns a `Result`.
 A `Result` can be constructed as either
 `Result.Success` or `Result.Failure`.
@@ -718,10 +768,12 @@ we can read this as
 "`ParseAwsKmsArn` succeeding implies
 that the called string was split into 6 parts"
 
-Now, go to the `duvet` report (compliance_report.html)
-and click on this requirement.
+Now, go back to the `duvet` report window (compliance_report.html)
+and click on this requirement
+(the first line with a red underline at the top of the page).
 You should get a popup.
-Click on the `IMPLICATION` tab
+Click on the `IMPLICATION` tab,
+which should briefly change to "IMPLICATION - COPIED!",
 and then paste right above the `ensures` clause!
 
 You should see an annotation
@@ -732,16 +784,16 @@ in the code that looks like this
 
     //= aws-kms-key-arn.txt#2.5
     //= type=implication
-    //# A string with 5 ":" that MUST delimit following 6 parts:
+    //# A valid AWS KMS ARN is a string with 5 ":" that MUST delimit the following 6 parts:
 
 ```
 
-1. `//=` and `//#`
+1. `//=` and `//#`:
 This is duvet!
 This is how we take our implementation
 and annotate so that we know we captured every requirement.
 
-1. `//= type=implication`
+1. `//= type=implication`:
 `duvet` wants us to annotate the implementation
 *and* provide some evidence that the implementation is correct.
 In Dafny an `ensures` clause MUST be true,
@@ -749,21 +801,21 @@ therefore this bounds the implementation
 and provides evidence of the implementation's correctness.
 If you used `duvet` in a more traditional language,
 we would have annotated the `Need` call
-writen a test and annotated that test.
+with a test and annotated that test.
 
 Run 
 ```bash
 make duvet_report
 ```
 
-and our report will have updated.
+and switch back to the report window, which should automatically refresh.
 This requirement is now green!
 
 ## Step 14
 
 Looking at our specification
 we can fill in several of our requirements.
-All of this syntax we have already gone over.
+Most of this syntax we have already gone over.
 
 <!-- !test check ParseAwsKmsArn all requirement -->
 ```dafny
@@ -773,12 +825,12 @@ All of this syntax we have already gone over.
 
     //= aws-kms-key-arn.txt#2.5
     //= type=implication
-    //# A string with 5 ":" that MUST delimit following 6 parts:
+    //# A valid AWS KMS ARN is a string with 5 ":" that MUST delimit the following 6 parts:
     ensures result.Success? ==> |Split(identifier, ':')| == 6
 
     //= aws-kms-key-arn.txt#2.5
     //= type=implication
-    //# MUST start with string "arn"
+    //# It MUST start with string "arn"
     ensures result.Success? ==> "arn" <= identifier
 
     //= aws-kms-key-arn.txt#2.5
@@ -808,14 +860,14 @@ All of this syntax we have already gone over.
 
 ```
 
+There's just one new feature to explain:
+
 1. `"arn" <= identifier`
-Since Dafny treats `string` as a sequence characters
-`<=` means "start with".
-This is probably a little surprising.
-But the only way for 2 sequences to be equal
-is if they are the same length
-and every element is the same in the same order.
-This bounds the "greater than" to adding any number of elements.
+Since Dafny treats `string` as a pure sequence of characters,
+`<=` means "starts with".
+This is probably a little surprising,
+but turns out to be the most convenient meaning
+when using sequences in Dafny specifications.
 
 But wait!
 Dafny is complaining:
@@ -823,13 +875,13 @@ The postcondition
 `ensures result.Success? ==> 0 < |Split(identifier, ':')[5]|`
 may not hold.
 
-Hum, obviously we need to update `ParseAwsKmsResources`
+Hmm, obviously we need to update `ParseAwsKmsResource`
 to return a `Result`.
 
-<!-- !test check ParseAwsKmsResources stub -->
+<!-- !test check ParseAwsKmsResource stub -->
 ```dafny
 
-  function ParseAwsKmsResources(arnResource: string)
+  function ParseAwsKmsResource(arnResource: string)
     : (result: Result<AwsKmsResource, string>)
 
 ```
@@ -839,27 +891,27 @@ Since we return a `Result` now.
 
 ```dafny
 
-    var resource :- ParseAwsKmsResources(components[5]);
+    var resource :- ParseAwsKmsResource(components[5]);
 
 ```
 
 Dafny is still complaining.
 Let's think about this.
-`ParseAwsKmsResources` does not have any `ensures` on it.
+`ParseAwsKmsResource` does not have any `ensures` on it.
 So Dafny is unable to make any connection
 between the `AwsKmsResource` and the input `string`.
 So let's fix that.
 
-<!-- !test check ParseAwsKmsResources all requirements -->
+<!-- !test check ParseAwsKmsResource all requirements -->
 ```dafny
 
-  function ParseAwsKmsResources(arnResource: string)
+  function ParseAwsKmsResource(arnResource: string)
     : (result: Result<AwsKmsResource, string>)
 
     //= aws-kms-key-arn.txt#2.5
     //= type=implication
     //# It MUST be split by a
-    //# single "/" any additional "/" are included in the resource id
+    //# single "/", with any any additional "/" included in the resource id
     ensures result.Success?
     ==>
       && '/' in arnResource
@@ -890,7 +942,7 @@ Now we show that Dafny will honor
 requirements on these stubs.
 Since Dafny will also force us
 to `ensure` these requirements in our implementation
-this kind of specification driven development
+this kind of specification-driven development
 is a powerful tool in our toolbox.
 
 Second, if we run
@@ -898,7 +950,7 @@ Second, if we run
 make duvet_report
 ```
 
-Now our report is complete.
+Now section 2.5 of our report is complete.
 Once we add an implementation
 to this `function` that Dafny will accept
 we are done with this section!
@@ -908,18 +960,18 @@ and see if you can work out why this is indeed enforced.
 
 ## Step 15
 
-Now we can add an implementation to `ParseAwsKmsResources`.
+Now we can add an implementation to `ParseAwsKmsResource`.
 
-<!-- !test check ParseAwsKmsResources full -->
+<!-- !test check ParseAwsKmsResource full -->
 ```dafny
 
-  function ParseAwsKmsResources(arnResource: string)
+  function ParseAwsKmsResource(arnResource: string)
     : (result: Result<AwsKmsResource, string>)
 
     //= aws-kms-key-arn.txt#2.5
     //= type=implication
     //# It MUST be split by a
-    //# single "/" any additional "/" are included in the resource id
+    //# single "/", with any any additional "/" included in the resource id
     ensures result.Success?
     ==>
       && '/' in arnResource
@@ -954,9 +1006,8 @@ Now we can add an implementation to `ParseAwsKmsResources`.
 
 1. `info[1..]`
 This is a slice notation.
-This will return a new sequence.
-It will include the second element.
-If you want more details see [here](https://dafny.org/dafny/DafnyRef/DafnyRef#sec-other-sequence-expressions)
+This will return a new sequence value identical to the original, but dropping the first element.
+If you want more details, see [here](https://dafny.org/dafny/DafnyRef/DafnyRef#sec-other-sequence-expressions).
 
 
 ## Step 16
@@ -967,7 +1018,7 @@ This is covered in sections 2.8 and 2.9.
 This adds some complexity.
 Since a raw key id is not a complete resource section.
 
-So let's throw up the last of our implementation as stubs
+So let's throw up the last of our implementation as stubs:
 
 <!-- !test check Identifier stubs -->
 ```dafny
@@ -979,7 +1030,7 @@ So let's throw up the last of our implementation as stubs
   function ParseAwsKmsIdentifier(identifier: string)
     : (result: Result<AwsKmsIdentifier, string>)
 
-  function ParseAwsKmsRawResources(identifier: string)
+  function ParseAwsKmsRawResource(identifier: string)
     : (result: Result<AwsKmsResource, string>)
 
   //= aws-kms-key-arn.txt#2.8
@@ -1023,7 +1074,7 @@ Let's go with "It starts with arn:".
       var arn :- ParseAwsKmsArn(identifier);
       Success(AwsKmsArnIdentifier(arn))
     else
-      var r :- ParseAwsKmsRawResources(identifier);
+      var r :- ParseAwsKmsRawResource(identifier);
       Success(AwsKmsRawResourceIdentifier(r))
   }
 
@@ -1031,16 +1082,16 @@ Let's go with "It starts with arn:".
 
 ## Step 18
 
-Lets do `ParseAwsKmsRawResources`.
+Lets do `ParseAwsKmsRawResource`.
 First we will do a quick naive implementation.
 
 ```dafny
 
-  function ParseAwsKmsRawResources(identifier: string)
+  function ParseAwsKmsRawResource(identifier: string)
     : (result: Result<AwsKmsResource, string>)
   {
     if "alias/" <= identifier then
-      ParseAwsKmsResources(identifier)
+      ParseAwsKmsResource(identifier)
     else
       :- Need(!("key/" <= identifier), "Malformed raw key id: " + identifier);
       var resource := AwsResource(
@@ -1053,14 +1104,14 @@ First we will do a quick naive implementation.
 
 ```
 
-Hum, so Dafny does not believe us.
+Hmm, so Dafny does not believe us.
 Let's see,
 does it believe
 ```dafny
 assert resource.resourceType == "key";
 ```
 
-Hum, so what is the other condition then?
+Hmm, so what is the other condition then?
 ```dafny
 assert 0 < |resource.value|;
 ```
@@ -1072,18 +1123,25 @@ from the `Success` to the `assert`.
 Where the Dafny error message is
 also gives us information we can use.
 
-Now we could use `ParseAwsKmsResources`
+This does NOT mean that the `Success` magically became correct!
+Dafny is just telling you that IF `0 < |resource.value|` is true,
+the return value is correct.
+It is important to keep in mind that all of these assertions are connected,
+and if any single assertion is not proven,
+it means you can't necessarily trust the proof of any others.
+
+Now we could use `ParseAwsKmsResource`
 but that has a bunch of redundant string operations.
 Let's just add the condition to our existing `Need`:
 
-<!-- !test check ParseAwsKmsRawResources complete -->
+<!-- !test check ParseAwsKmsRawResource complete -->
 ```dafny
 
-  function ParseAwsKmsRawResources(identifier: string)
+  function ParseAwsKmsRawResource(identifier: string)
     : (result: Result<AwsKmsResource, string>)
   {
     if "alias/" <= identifier then
-      ParseAwsKmsResources(identifier)
+      ParseAwsKmsResource(identifier)
     else
       :- Need(!("key/" <= identifier) && 0 < |identifier|, "Malformed raw key id: " + identifier);
       var resource := AwsResource(
@@ -1118,7 +1176,7 @@ First `MultiRegionAwsKmsArn?`
 
     //= aws-kms-key-arn.txt#2.8
     //= type=implication
-    //# If resource type is "key" and resource ID starts with
+    //# If the resource type is "key" and the resource ID starts with
     //# "mrk-", this is a AWS KMS multi-Region key ARN and MUST return true.
     ensures
       && arn.resource.resourceType == "key"
@@ -1128,7 +1186,7 @@ First `MultiRegionAwsKmsArn?`
 
     //= aws-kms-key-arn.txt#2.8
     //= type=implication
-    //# If resource type is "key" and resource ID does not start with "mrk-",
+    //# If the resource type is "key" and the resource ID does not start with "mrk-",
     //# this is a (single-region) AWS KMS key ARN and MUST return false.
     ensures
       && arn.resource.resourceType == "key"
@@ -1153,7 +1211,7 @@ it does not know anything about `MultiRegionAwsKmsResource?`.
 Let's just add it this time.
 
 This is always a `key` that starts with `mrk-`.
-Given everything we have learned we have learned:
+Given everything we have learned we have:
 
 <!-- !test check MultiRegionAwsKmsResource? -->
 ```dafny
@@ -1172,7 +1230,7 @@ and see that these conditions would be correct.
 This transparency of `function`s can be powerful.
 But Dafny can not unroll every function.
 
-Finally `MultiRegionAwsKmsIdentifier?`!!
+Finally, `MultiRegionAwsKmsIdentifier?`!
 
 <!-- !test check MultiRegionAwsKmsIdentifier? -->
 ```dafny
@@ -1192,18 +1250,20 @@ Finally `MultiRegionAwsKmsIdentifier?`!!
 
 ```
 
-The `match` expression.
-This looks at they possible constructors of `AwsKmsIdentifier`
+This `match` expression looks at the possible constructors of `AwsKmsIdentifier`
 and creates a branch for each one.
 If say `AwsKmsArnIdentifier` had more arguments,
 then we would be required to list them all.
-These arguments the bind variables that are in scope
+The arguments bind variables that are in scope
 in that `case` branch.
 
 ## Step 20
 
 Wait!
-Run `make duvet_report`.
+Run `make duvet_report` and notice the command still fails.
+Click "Compliance Coverage Report" in the header bar of the report
+to navigate back to the top.
+
 We are missing some proof.
 Section 2.9.
 
@@ -1255,7 +1315,7 @@ we want to deal with every string that could be a `AwsKmsIdentifier`.
 
 For this we need a precondition.
 Something that MUST be true *before* the function is evaluated.
-Dafny expresses this with the keyword `requires`
+Dafny expresses this with the keyword `requires`:
 
 <!-- !test check MultiRegionAwsKmsIdentifier?Correct with requires -->
 ```dafny
@@ -1267,7 +1327,7 @@ Dafny expresses this with the keyword `requires`
 
 Now everywhere we can assume that the string `s`
 is a valid `AwsKmsIdentifier`!
-This simplifies our first requirement
+This simplifies our first requirement:
 
 <!-- !test check MultiRegionAwsKmsIdentifier?Correct first ensures -->
 ```dafny
@@ -1278,8 +1338,7 @@ This simplifies our first requirement
     //= aws-kms-key-arn.txt#2.9
     //= type=implication
     //# If the input starts with "arn:", this MUST return the output of
-    //# identifying an an AWS KMS multi-Region ARN (aws-kms-key-
-    //# arn.md#identifying-an-an-aws-kms-multi-region-arn) called with this
+    //# identifying an an AWS KMS multi-Region ARN (Section 2.8) called with this
     //# input.
     ensures "arn:" <= identifier
       ==>
@@ -1361,8 +1420,7 @@ Putting that all together we get.
     //= aws-kms-key-arn.txt#2.9
     //= type=implication
     //# If the input starts with "arn:", this MUST return the output of
-    //# identifying an an AWS KMS multi-Region ARN (aws-kms-key-
-    //# arn.md#identifying-an-an-aws-kms-multi-region-arn) called with this
+    //# identifying an an AWS KMS multi-Region ARN (Section 2.8) called with this
     //# input.
     ensures "arn:" <= identifier
       ==>
@@ -1405,4 +1463,34 @@ Putting that all together we get.
 
 ## Step 21
 
-TODO run duvet with a CI so that we can see the exit code.
+Let's run Duvet one last time:
+
+```bash
+make duvet_report
+```
+
+Success! The command no longer fails
+(if you don't believe the lack of error messages, you can check with `echo $?`)
+and the report is a happy sea of green.
+Congratulations on your formally-verified implementation!
+
+## Extra Credit
+
+Here are a couple of bonus questions if you are hungry for more:
+
+1. If you have strong instincts to keep your code DRY,
+   you might feel uncomfortable with all of the repeated `0 < | ... |`
+   expressions everywhere we require a non-empty string.
+   Try defining a `NonEmptyString` subset type and use it
+   in place of `string` wherever it makes sense to tighten things up.
+   Where should the relevant Duvet citations move to?
+   
+2. Now that we have implemented parsing, 
+   try implementing the other direction in a `AwsKmsIdentifierToString`
+   function and write a lemma to prove that it is always
+   the inverse of `ParseAwsKmsIdentifier`.
+   You will find one possible solution [here](../exercises/complete/src/SoundnessVsCompletness.dfy).
+
+3. `Split` and `Join` are relatively simple functions.
+    Try replacing the functions we gave you with your own. 
+    If you really want to flex, get it to verify *before* writing your implementation.
